src/PlutusIR/Semantics/TypeSafety/SubstitutionPreservesTyping/TermSubstitution.v
@@ -307,7 +307,7 @@ Proof with eauto.
   - (* TyAbs *)
     simpl.
     inversion H0; subst.
-    apply T_TyAbs.
+    apply T_TyAbs; auto.
     unfold P_Term in H.
     eapply H; eauto.
     (* s not free in U by [],,[] |-+ v : Un 
